@prefix a-dd:  <https://w3id.org/arco/ontology/denotative-description/> .
@prefix arco:  <https://w3id.org/arco/ontology/arco/> .
@prefix opla:  <http://ontologydesignpatterns.org/opla/> .
@prefix owl:   <http://www.w3.org/2002/07/owl#> .
@prefix rdf:   <http://www.w3.org/1999/02/22-rdf-syntax-ns#> .
@prefix a-loc: <https://w3id.org/arco/ontology/location/> .
@prefix odp-pat: <http://www.ontologydesignpatterns.org/cp/owl/> .
@prefix rdfs:  <http://www.w3.org/2000/01/rdf-schema#> .

a-loc:isTimeIndexedTypedLocationOf
        owl:inverseOf  a-loc:hasTimeIndexedTypedLocation .

odp-pat:atTime  rdfs:domain  a-loc:TimeIndexedTypedLocation , odp-pat:TimeIndexedSituation ;
        rdfs:range          <https://w3id.org/italia/onto/TI/TimeInterval> ;
        rdfs:subPropertyOf  odp-pat:isSettingFor .

odp-pat:hasPart  owl:inverseOf  odp-pat:isPartOf .

odp-pat:part-of  a    opla:Pattern ;
        rdfs:comment  "The pattern represents entities and their parts i.e., part-whole relations, with transitivity. Explore instances of this pattern to get information of a thing and the parts its composed by." ;
        rdfs:label    "Part Of" .

a-dd:hasMeasurement  rdfs:domain  a-dd:MeasurementCollection ;
        rdfs:range   a-dd:Measurement .

odp-pat:collection  a  opla:Pattern ;
        rdfs:comment  "The pattern is a basic one: it catches the idea of a collection and its members. It represents a collection and members of a collection. Explore the instances to see information about the collection and its member." ;
        rdfs:label    "Collection" .

arco:hasCulturalPropertyComponent
        rdfs:subPropertyOf  odp-pat:hasPart ;
        owl:inverseOf       arco:isCulturalPropertyComponentOf .

arco:isCulturalPropertyComponentOf
        rdfs:subPropertyOf  odp-pat:isPartOf .

arco:CulturalPropertyComponent
        rdfs:domain  arco:isCulturalPropertyComponentOf ;
        rdfs:range   arco:ComplexCulturalProperty .

odp-pat:hasMember  rdfs:domain  odp-pat:Collection ;
        rdfs:range   owl:Thing .

<https://w3id.org/italia/onto/TI/hasIntervalDate>
        a            owl:DatatypeProperty ;
        rdfs:domain  <https://w3id.org/italia/onto/TI/TimeInterval> .

odp-pat:time-interval
        a                        opla:Pattern ;
        rdfs:comment             "This pattern represents an interval of time." ;
        rdfs:label               "Time Interval" ;
        opla:componentOfPattern  a-loc:time-indexed-typed-location , odp-pat:time-indexed-situation .

odp-pat:hasTimeIndexedSetting
        rdfs:domain         owl:Thing ;
        rdfs:range          odp-pat:TimeIndexedSituation ;
        rdfs:subPropertyOf  odp-pat:hasSetting .

owl:Thing  rdfs:domain  odp-pat:isPartOf , odp-pat:hasPart ;
        rdfs:range   owl:Thing .

a-dd:measurement-collection
        a                             opla:Pattern ;
        rdfs:comment                  "The pattern represents a collection of measurement of an cultural property. Some type of measurement for a cultural property are height, width, length, weight... Explore the instances of the pattern to view data relatives to measurements collected about a cultural property." ;
        rdfs:label                    "Cultural Property Measurements" ;
        opla:specializationOfPattern  odp-pat:collection .

odp-pat:isSettingFor  owl:inverseOf  odp-pat:hasSetting .

a-loc:cultural-property-component-of
        a                             opla:Pattern ;
        rdfs:comment                  "The pattern represents complex cultural properties and components of the cultural property. For example it may represent a building (like a church) and their architectural elements. Or a painting and details of it. Explore the instances of this pattern to get information about a complex cultural property and components it's made by." ;
        rdfs:label                    "Cultural Property Components" ;
        opla:specializationOfPattern  odp-pat:part-of .

<https://w3id.org/italia/onto/TI/hasIntervalEndDate>
        a                   owl:DatatypeProperty ;
        rdfs:subPropertyOf  <https://w3id.org/italia/onto/TI/hasIntervalDate> .

arco:ComplexCulturalProperty
        rdfs:domain  arco:hasCulturalPropertyComponent ;
        rdfs:range   arco:CulturalPropertyComponent .

odp-pat:hasSetting  rdfs:domain  owl:Thing ;
        rdfs:range   odp-pat:Situation .

a-loc:hasTimeIndexedTypedLocation
        rdfs:domain         a-loc:CulturalProperty ;
        rdfs:range          a-loc:TimeIndexedTypedLocation ;
        rdfs:subPropertyOf  odp-pat:hasSetting ;
        owl:inverseOf       a-loc:isTimeIndexedTypedLocationOf .

odp-pat:isTimeIndexFor
        owl:inverseOf  odp-pat:hasTimeIndexedSetting .

odp-pat:time-indexed-situation
        a                             opla:Pattern ;
        rdfs:comment                  "The pattern represents time indexed situations. This pattern adds a time specification (the Time interval pattern) to the Situation pattern. It represents situations, things contextualized and the time interval in which the situation occured. Explore the instances of this pattern to view data a situation, things involved and the time interval in which situation happened." ;
        rdfs:label                    "Time Indexed Situation" ;
        opla:specializationOfPattern  odp-pat:situation .

odp-pat:TimeIndexedSituation
        rdfs:subClassOf  odp-pat:Situation .

a-dd:MeasurementCollection
        rdfs:subClassOf  <http://www.ontologydesignpatterns.org/cp/owl/collectionentity.owl#Collection> .

<https://w3id.org/italia/onto/TI/hasIntervalStartDate>
        a                   owl:DatatypeProperty ;
        rdfs:subPropertyOf  <https://w3id.org/italia/onto/TI/hasIntervalDate> .

a-loc:TimeIndexedTypedLocation
        rdfs:subClassOf  odp-pat:TimeIndexedSituation .

a-loc:time-indexed-typed-location
        a                             opla:Pattern ;
        rdfs:comment                  "The pattern represents time indexed typed locations. This pattern represents locations of a cultural property at a specified time interval. Location have a specified type. For example the Current Location of a cultural property or the previous location of a cultural property and the time period during which the cultural property has been in the specified location. Explore instances of this pattern to get information about the location of a cultural property and the time period since it is in that location or has been in the past." ;
        rdfs:label                    "Cultural Property Locations" ;
        opla:specializationOfPattern  odp-pat:time-indexed-situation .

odp-pat:situation  a  opla:Pattern ;
        rdfs:comment  "The pattern represents contexts or situations, and the things that are contextualized. Explore the instances to get information about a situation and the things invlolved in that situation." ;
        rdfs:label    "Situation" .
