@prefix a-dd:  <https://w3id.org/arco/ontology/denotative-description/> .
@prefix arco:  <https://w3id.org/arco/ontology/arco/> .
@prefix opla:  <http://ontologydesignpatterns.org/opla/> .
@prefix owl:   <http://www.w3.org/2002/07/owl#> .
@prefix rdf:   <http://www.w3.org/1999/02/22-rdf-syntax-ns#> .
@prefix a-loc: <https://w3id.org/arco/ontology/location/> .
@prefix odp-pat: <http://www.ontologydesignpatterns.org/cp/owl/> .
@prefix rdfs:  <http://www.w3.org/2000/01/rdf-schema#> .

a-loc:isTimeIndexedTypedLocationOf
        owl:inverseOf  a-loc:hasTimeIndexedTypedLocation .

odp-pat:atTime  rdfs:domain  a-loc:TimeIndexedTypedLocation , odp-pat:TimeIndexedSituation ;
        rdfs:range          <https://w3id.org/italia/onto/TI/TimeInterval> ;
        rdfs:subPropertyOf  odp-pat:isSettingFor .

odp-pat:hasPart  owl:inverseOf  odp-pat:isPartOf .

odp-pat:part-of  a    opla:Pattern ;
        rdfs:comment  "This Content OP allows designers to represent entities and their parts i.e., part-whole relations, with transitivity." ;
        rdfs:label    "Part Of" .

a-dd:hasMeasurement  rdfs:domain  a-dd:MeasurementCollection ;
        rdfs:range   a-dd:Measurement .

odp-pat:collection  a  opla:Pattern ;
        rdfs:comment  "This pattern is a basic one: it catches the idea of a collection and its members." ;
        rdfs:label    "Collection" .

arco:hasCulturalPropertyComponent
        rdfs:subPropertyOf  odp-pat:hasPart ;
        owl:inverseOf       arco:isCulturalPropertyComponentOf .

arco:isCulturalPropertyComponentOf
        rdfs:subPropertyOf  odp-pat:isPartOf .

arco:CulturalPropertyComponent
        rdfs:domain  arco:isCulturalPropertyComponentOf ;
        rdfs:range   arco:ComplexCulturalProperty .

odp-pat:hasMember  rdfs:domain  odp-pat:Collection ;
        rdfs:range   owl:Thing .

<https://w3id.org/italia/onto/TI/hasIntervalDate>
        a            owl:DatatypeProperty ;
        rdfs:domain  <https://w3id.org/italia/onto/TI/TimeInterval> .

odp-pat:time-interval
        a                        opla:Pattern ;
        rdfs:comment             "This pattern represents an interval of time" ;
        rdfs:label               "Time Interval" ;
        opla:componentOfPattern  a-loc:time-indexed-typed-location , odp-pat:time-indexed-situation .

odp-pat:hasTimeIndexedSetting
        rdfs:domain         owl:Thing ;
        rdfs:range          odp-pat:TimeIndexedSituation ;
        rdfs:subPropertyOf  odp-pat:hasSetting .

owl:Thing  rdfs:domain  odp-pat:hasPart , odp-pat:isPartOf ;
        rdfs:range   owl:Thing .

a-dd:measurement-collection
        a                             opla:Pattern ;
        rdfs:comment                  "This pattern represents a collection of measurement of an object" ;
        rdfs:label                    "Measurement Collection" ;
        opla:specializationOfPattern  odp-pat:collection .

odp-pat:isSettingFor  owl:inverseOf  odp-pat:hasSetting .

a-loc:cultural-property-component-of
        a                             opla:Pattern ;
        rdfs:comment                  "This Content OP allows designers to represent cultural properties and their components or parts." ;
        rdfs:label                    "Cultural Property Component Of" ;
        opla:specializationOfPattern  odp-pat:part-of .

<https://w3id.org/italia/onto/TI/hasIntervalEndDate>
        a                   owl:DatatypeProperty ;
        rdfs:subPropertyOf  <https://w3id.org/italia/onto/TI/hasIntervalDate> .

arco:ComplexCulturalProperty
        rdfs:domain  arco:hasCulturalPropertyComponent ;
        rdfs:range   arco:CulturalPropertyComponent .

a-loc:hasTimeIndexedTypedLocation
        rdfs:domain         a-loc:CulturalProperty ;
        rdfs:range          a-loc:TimeIndexedTypedLocation ;
        rdfs:subPropertyOf  odp-pat:hasSetting ;
        owl:inverseOf       a-loc:isTimeIndexedTypedLocationOf .

odp-pat:hasSetting  rdfs:domain  owl:Thing ;
        rdfs:range   odp-pat:Situation .

odp-pat:isTimeIndexFor
        owl:inverseOf  odp-pat:hasTimeIndexedSetting .

odp-pat:time-indexed-situation
        a                             opla:Pattern ;
        rdfs:comment                  "To represent time indexed situations. This pattern adds a time specification (the Time interval pattern) to the Situation pattern, in order to provide a handy solution to many cases. " ;
        rdfs:label                    "Time Indexed Situation" ;
        opla:specializationOfPattern  odp-pat:situation .

odp-pat:TimeIndexedSituation
        rdfs:subClassOf  odp-pat:Situation .

a-dd:MeasurementCollection
        rdfs:subClassOf  <http://www.ontologydesignpatterns.org/cp/owl/collectionentity.owl#Collection> .

<https://w3id.org/italia/onto/TI/hasIntervalStartDate>
        a                   owl:DatatypeProperty ;
        rdfs:subPropertyOf  <https://w3id.org/italia/onto/TI/hasIntervalDate> .

a-loc:TimeIndexedTypedLocation
        rdfs:subClassOf  odp-pat:TimeIndexedSituation .

a-loc:time-indexed-typed-location
        a                             opla:Pattern ;
        rdfs:comment                  "To represent time indexed typed locations. This pattern represents locations of a defined type and a time specification" ;
        rdfs:label                    "Time Indexed Typed Location" ;
        opla:specializationOfPattern  odp-pat:time-indexed-situation .

odp-pat:situation  a  opla:Pattern ;
        rdfs:comment  "To represent contexts or situations, and the things that are contextualized." ;
        rdfs:label    "Situation" .
